code/ecdsap256sha2/Hacl.Impl.ECDSA.fsti
@@ -188,9 +188,8 @@ val ecdsa_verification_blake2:
       result == Spec.ECDSA.ecdsa_verification_blake2 (publicKeyX, publicKeyY) r s (v mLen) (as_seq h0 m))
 
 
-val ecdsa_verification_blake2hl:
-  mLen:size_t
-  -> m:lbuffer uint8 mLen 
+val ecdsa_verification_without_hash:
+  m:lbuffer uint8 (size 32) 
   -> pubKey:lbuffer uint8 (size 64)
   -> r:lbuffer uint8 (size 32)
   -> s:lbuffer uint8 (size 32)
@@ -203,7 +202,7 @@ val ecdsa_verification_blake2hl:
       let r = nat_from_bytes_be (as_seq h1 r) in
       let s = nat_from_bytes_be (as_seq h1 s) in
       modifies0 h0 h1 /\
-      result == Spec.ECDSA.ecdsa_verification_blake2 (publicKeyX, publicKeyY) r s (v mLen) (as_seq h0 m))
+      result == Spec.ECDSA.ecdsa_verification_without_hash (publicKeyX, publicKeyY) r s  (as_seq h0 m))
 
 
 
